TwoLevel.v
@@ -1,0 +1,643 @@
+Require Import DataTypes Induction.
+Require Import Channel Cache Compatible L1.
+
+Module dt <: DataTypes.
+  Parameter classical: forall P, P \/ ~ P.
+
+  Parameter Addr: Set.
+  Inductive Desc := Ld | St.
+
+  Definition Index := nat.
+
+  Inductive Cache': Set :=
+    | Parent : Cache'
+    | Child : nat -> Cache'.
+
+  Definition Cache := Cache'. 
+
+  Definition parent c p := 
+    match c with
+      | Parent => False
+      | Child _ => 
+        match p with
+          | Parent => True
+          | Child _ => False
+        end
+    end.
+
+  Definition leaf x := match x with
+                         | Parent => False
+                         | Child _ => True
+                       end.
+
+  Theorem noChildIsParent: forall {c}, leaf c -> forall c', ~ parent c' c.
+  Proof.
+    intros c leafC.
+    unfold leaf in leafC.
+    destruct c.
+    firstorder.
+    unfold not; intros c' parentc'.
+    unfold parent in parentc'.
+    destruct c'; assumption.
+  Qed.
+
+  Theorem noParentHasParent: forall c, ~ parent Parent c.
+  Proof.
+    unfold not; intros c parentc.
+    unfold parent in parentc.
+    assumption.
+  Qed.
+    
+  Theorem whoParent: forall n, parent (Child n) Parent.
+  Proof.
+    intros.
+    unfold parent.
+    auto.
+  Qed.
+
+  Theorem who'Parent: forall c, leaf c -> parent c Parent.
+  Proof.
+    intros c leaf_c.
+    destruct c; unfold leaf; auto.
+  Qed.
+
+  Parameter descendent: Cache -> Cache -> Prop.
+
+  Inductive State := In | Sh | Mo.
+
+  Definition slt x y := match x with
+                          | In => match y with
+                                    | In => False
+                                    | Sh => True
+                                    | Mo => True
+                                  end
+                          | Sh => match y with
+                                    | In => False
+                                    | Sh => False
+                                    | Mo => True
+                                  end
+                          | Mo => False
+                        end.
+  Definition sgt x y := slt y x.
+  Definition sle x y := match x with
+                          | In => match y with
+                                    | In => True
+                                    | Sh => True
+                                    | Mo => True
+                                  end
+                          | Sh => match y with
+                                    | In => False
+                                    | Sh => True
+                                    | Mo => True
+                                  end
+                          | Mo => match y with
+                                    | In => False
+                                    | Sh => False
+                                    | Mo => True
+                                  end
+                        end.
+
+  Theorem sle_eq: forall {x y}, x = y -> sle x y.
+  Proof.
+    intros x y x_eq_y. rewrite x_eq_y.
+    unfold sle.
+    destruct y; auto.
+  Qed.
+
+  Theorem slt_neq: forall {x y}, x = y -> ~ slt x y.
+  Proof.
+    intros x y x_eq_y. rewrite x_eq_y. intros geez.
+    unfold slt in geez.
+    destruct y; auto.
+  Qed.
+
+  Theorem slt_neq': forall {x y}, slt x y -> x <> y.
+  Proof.
+    unfold slt; destruct x; destruct y; auto; discriminate.
+  Qed.
+
+  Theorem slt_slti_false: forall {x y}, slt x y -> slt y x -> False.
+  Proof.
+    intros x y slt1 slt2.
+    unfold slt in *; destruct x in *; destruct y in *; auto.
+  Qed.
+
+  Theorem slt_slei_false: forall {x y}, slt x y -> sle y x -> False.
+  Proof.
+    intros x y s1 s2.
+    unfold slt in *; unfold sle in *; destruct x in *; destruct y in *; auto.
+  Qed.
+
+  Theorem not_slt_sle: forall {x y}, ~ slt x y -> sle y x.
+  Proof.
+    intros x y noSlt.
+    unfold sle; unfold slt in *;
+    destruct x; destruct y; auto.
+  Qed.
+
+  Theorem not_sle_slt: forall {x y}, ~ sle x y -> slt y x.
+  Proof.
+    intros x y noSle.
+    unfold sle in *; unfold slt in *;
+    destruct x; destruct y; auto.
+  Qed.
+
+  Theorem slt_eq_slt_dec: forall {x y}, slt x y \/ x = y \/ slt y x.
+  Proof.
+    intros x y.
+    destruct x; destruct y; unfold slt; auto.
+  Qed.
+
+  Theorem slt_eq_sle: forall {x y}, sle x y = slt x y \/ x = y.
+  Proof.
+    intros x y.
+    unfold sle; unfold slt.
+    destruct x; destruct y; auto.
+  Qed.
+    
+
+  Definition Time := nat.
+  Parameter state: Cache -> Addr -> Time -> State.
+  Parameter dir: Cache -> Cache -> Addr -> Time -> State.
+
+  Parameter Mesg: Set.
+  Parameter from: Mesg -> State.
+  Parameter to: Mesg -> State.
+  Parameter addr: Mesg -> Addr.
+
+  Parameter ChannelType: Set.
+
+  Parameter mch rch: ChannelType.
+
+  Parameter Label : Set.
+  Inductive StLabel := Initial | Store : Label -> StLabel.
+  Parameter data: Cache -> Addr -> Time -> StLabel.
+  Parameter dataM: Mesg -> StLabel.
+
+End dt.
+
+
+Module Type LatestValueAxioms (ch: ChannelPerAddr dt) (l1: L1Axioms dt).
+  Import dt ch l1.
+
+  Axiom toChild: forall {n a t p m},
+                   parent n p -> 
+                   mark mch p n a t m -> from m = In -> dataM m = data p a t.
+  Axiom fromParent: forall {n a t p m},
+                      parent n p -> 
+                      recv mch p n a t m -> from m = In -> data n a (S t) = dataM m.
+  Axiom toParent: forall {n a t c m},
+                     parent c n ->
+                     mark mch c n a t m -> slt Sh (from m) -> dataM m = data c a t.
+  Axiom fromChild: forall {n a t c m},
+                     parent c n ->
+                     recv mch c n a t m -> slt Sh (from m) -> data n a (S t) = dataM m.
+  Axiom initLatest: forall {n} a, (forall {p}, ~ parent n p) -> data n a 0 = Initial
+                                                                /\ state n a 0 = Mo.
+
+  Axiom deqImpData: forall {n a t l i}, deqR n l a St i t -> data n a (S t) = Store l.
+
+  Axiom changeData:
+    forall {n a t},
+      data n a (S t) <> data n a t ->
+      (exists m, (exists p, parent n p /\ recv mch p n a t m /\ from m = In) \/
+                 (exists c, parent c n /\ recv mch c n a t m /\ slt Sh (from m))) \/
+      exists l i, deqR n l a St i t.
+End LatestValueAxioms.
+
+Module LatestValueTheorems (ch: ChannelPerAddr dt) (c: BehaviorAxioms dt ch)
+       (l1: L1Axioms dt) (comp: CompatBehavior dt ch) (lv: LatestValueAxioms ch l1).
+  Module mbt := mkBehaviorTheorems dt ch c.
+  Module cbt := mkCompat dt ch comp c.
+  Import dt ch c l1 comp lv mbt cbt.
+
+  Theorem uniqM:
+    forall {c a t},
+      leaf c ->
+      state c a t = Mo -> forall {co}, leaf co -> c <> co -> state co a t = In.
+  Proof.
+    intros c a t leaf_c c_M co leaf_co c_ne_co.
+    pose proof (who'Parent c leaf_c) as c_parent.
+    pose proof (who'Parent co leaf_co) as co_parent.
+    pose proof (conservative c_parent a t) as cLe.
+    pose proof (conservative co_parent a t) as coLe.
+    pose proof (@compatible Parent a t c c_parent) as [_ comp].
+    assert (dirM: dir Parent c a t = Mo) by
+        ( unfold sle in *; destruct (state c a t); destruct (dir Parent c a t); firstorder;
+          discriminate).
+    assert (co_ne_c: co <> c) by auto.
+    specialize (comp co co_ne_c co_parent).
+    rewrite dirM in comp.
+    unfold sle in *; destruct (dir Parent co a t); destruct (state co a t); firstorder.
+  Qed.
+
+  Section ForAddr.
+    Context {a: Addr}.
+    Theorem allLatestValue: forall {t n},
+      (sle Sh (state n a t) /\ forall {c}, parent c n -> sle (dir n c a t) Sh) ->
+      match data n a t with
+        | Initial => forall {ti}, 0 <= ti < t -> forall {ci li ii}, ~ deqR ci li a St ii ti
+        | Store lb =>
+          exists cb ib tb, tb < t /\ deqR cb lb a St ib tb /\
+                           forall {ti}, tb < ti < t ->
+                                        forall {ci li ii}, ~ deqR ci li a St ii ti
+      end.
+    Proof.
+      pose (fun t => forall n,
+              sle Sh (state n a t) /\
+              (forall c, parent c n -> sle (dir n c a t) Sh) ->
+                         match data n a t with
+                           | Initial =>
+                             forall ti : nat,
+                               0 <= ti < t ->
+                               forall (ci : Cache) (li : Label) (ii : Index),
+                                 ~ deqR ci li a St ii ti
+                           | Store lb =>
+                             exists (cb : Cache) (ib : Index) (tb : nat),
+                               tb < t /\
+                               deqR cb lb a St ib tb /\
+                               (forall ti : nat,
+                                  tb < ti < t ->
+                                  forall (ci : Cache) (li : Label) (ii : Index),
+                                    ~ deqR ci li a St ii ti)
+                         end) as P.
+      pose proof (initLatest a noParentHasParent) as [pInit pM].
+      apply (@ind P).
+      unfold P in *; clear P.
+      assert (childIn: forall n, state (Child n) a 0 = In).
+      intros c.
+      assert (pChilds: parent (Child c) Parent) by
+          (unfold parent; auto).
+      pose proof (initCompat pChilds a) as dirIn.
+      pose proof (conservative pChilds a 0) as sleSt.
+      unfold sle in *; destruct (dir Parent (Child c) a 0); destruct (state (Child c) a 0);
+      firstorder; discriminate.
+      intros n.
+      induction n.
+      rewrite pInit.
+      unfold not; intros.
+      assert (ti0: ti = 0) by omega.
+      rewrite ti0 in *.
+      pose proof (deqLeaf H1) as leafC.
+      unfold leaf in leafC.
+      destruct ci.
+      assumption.
+      specialize (childIn n).
+      pose proof (processDeq H1) as contra.
+      rewrite childIn in contra.
+      discriminate.
+      specialize (childIn n).
+      intros H.
+      rewrite childIn in H.
+      unfold sle in *; firstorder.
+      unfold P in *; clear P.
+      intros t SIHt n H.
+      assert (stEq: forall t, state Parent a t = Mo) by
+          (intros t'; pose proof (noParentNoStChange a t' noParentHasParent); rewrite <- pM in *;
+          auto).
+      destruct n.
+      destruct (classical (forall c, parent c Parent -> sle (dir Parent c a t) Sh)) as
+          [prevLatest|prevNotLatest].
+      assert (stM: sle Sh (state Parent a t)) by (specialize (stEq t);
+                                                   rewrite stEq; unfold sle; auto).
+      assert (cond: t <= t) by omega.
+      specialize (SIHt t cond Parent (conj stM prevLatest)); clear cond stM.
+      destruct H as [_ dirSmall].
+      assert (cSmall: forall c, parent c Parent -> sle (state c a t) Sh).
+      intros c c_child.
+      specialize (prevLatest c c_child).
+      pose proof (conservative c_child a t) as help.
+      unfold sle in *; destruct (state c a t); destruct (dir Parent c a t); auto.
+      assert (noDeq: forall ci li ii, ~ deqR ci li a St ii t) by
+          (unfold not; intros ci li ii H;
+           pose proof (processDeq H) as sth; simpl in *;
+                                             pose proof (deqLeaf H) as leaf_ci;
+           assert (ci_child: parent ci Parent) by (unfold parent; unfold leaf in *;
+                                                                  destruct ci; auto);
+           specialize (cSmall ci ci_child); rewrite sth in cSmall; unfold sle; auto).
+      destruct (classical (data Parent a (S t) = data Parent a t)) as [e1|e2].
+      rewrite e1.
+      destruct (data Parent a t).
+      intros ti cond.
+      assert (H: 0 <= ti < t \/ ti = t) by omega.
+      destruct H as [one|two]; [firstorder| rewrite two in *; firstorder].
+      destruct SIHt as [cb [ib [tb [tb_lt_t [deqTb rest]]]]].
+      exists cb; exists ib; exists tb.
+      assert (sth: tb < S t) by omega.
+      constructor.
+      assumption.
+      constructor.
+      assumption.
+      intros ti cond.
+      assert (H: tb < ti < t \/ ti = t) by omega.
+      destruct H as [one|two].
+      apply (rest ti one).
+      rewrite two in *; assumption.
+      pose proof (changeData e2) as sth.
+      destruct sth as [sth|deqSth].
+      destruct sth as [m [[p [parentp _]]|recvFromC]].
+      pose proof (noParentHasParent p parentp).
+      firstorder.
+      destruct recvFromC as [c [c_child [recvm sltFromM]]].
+      pose proof (recvmCond c_child recvm) as contra.
+      specialize (prevLatest c c_child).
+      rewrite <- contra in prevLatest.
+      unfold sle in *; unfold slt in *; destruct (from m); firstorder; discriminate.
+      destruct deqSth as [l [i deqSth]].
+      pose proof (deqLeaf deqSth) as H.
+      unfold leaf in H; firstorder.
+      destruct (classical (exists c, parent c Parent /\ ~ sle (dir Parent c a t) Sh))
+               as [[c [c_child dirHigh]]|notEx].
+      destruct H as [_ cacheLow].
+      specialize (cacheLow c c_child).
+      assert (downgrade: slt (dir Parent c a (S t)) (dir Parent c a t)) by
+          (unfold slt in *; unfold sle in *; destruct (dir Parent c a (S t));
+           destruct (dir Parent c a t); auto).
+      pose proof (slt_neq' downgrade) as neq.
+      pose proof (change (dt c_child) neq) as [[m markm] | [m recvm]].
+      pose proof (pSendUpgrade c_child markm) as upg.
+      pose proof (slt_slti_false downgrade upg) as f.
+      firstorder.
+      pose proof (recvImpMark recvm) as [ts [ts_le_t sendm]].
+
+
+
+      assert (pHigh: forall tx, ts <= tx < S t -> ~ sle (dir Parent c a tx) In) by admit.
+      assert (cLow: forall tx, ts <= tx < S t -> slt (state c a tx) Mo) by admit.
+
+
+
+      assert (others: forall tx, ts <= tx < S t ->
+                                 forall c', c' <> c -> parent c' Parent ->
+                                            sle (dir Parent c' a tx)
+                                                match dir Parent c a tx with
+                                                  | In => Mo
+                                                  | Sh => Sh
+                                                  | Mo => In
+                                                end) by
+          (intros tx _; apply (compatible a tx c_child)).
+      assert (c'DirLow:
+                forall tx,
+                  ts <= tx < S t -> 
+                  forall c', c' <> c -> parent c' Parent -> slt (dir Parent c' a tx) Mo).
+      intros tx cond c' c'_ne_c c'_child.
+      specialize (others tx cond c' c'_ne_c c'_child).
+      specialize (pHigh tx cond).
+      unfold slt in *; destruct (dir Parent c a tx); destruct (dir Parent c' a tx); auto.
+      assert (c'Low: forall tx, ts <= tx < S t -> forall c',
+                                                   c' <> c ->
+                                                   parent c' Parent ->
+                                                   slt (state c' a tx) Mo).
+      intros tx cond c' c'_ne_c c'_child.
+      specialize (c'DirLow tx cond c' c'_ne_c c'_child).
+      pose proof (conservative c'_child a tx) as sig.
+      unfold slt in *; destruct (dir Parent c' a tx); destruct (state c' a tx); auto.
+      assert (allLow: forall tx, ts <= tx < S t -> forall c0,
+                                           parent c0 Parent -> slt (state c0 a tx) Mo).
+      intros tx cond c0 c0_child.
+      assert (cache: {c0 = c} + {c0 <> c}) by (
+                                        decide equality;
+                                        decide equality).
+      destruct cache as [eq|notEq].
+      rewrite eq in *; apply (cLow tx cond).
+      apply (c'Low tx cond c0 notEq c0_child).
+      assert (noSt: forall ti, ts <= ti < S t ->
+                               forall ci li ii, ~ deqR ci li a St ii ti).
+      unfold not; intros ti cond ci li ii deqSt.
+      pose proof (deqLeaf deqSt) as leafCi.
+      assert(ci_child: parent ci Parent) by (unfold leaf in *; unfold parent in *; auto).
+      pose proof (processDeq deqSt) as mustMo.
+      simpl in *.
+      specialize (allLow ti cond ci ci_child).
+      unfold sle in allLow; destruct (state ci a ti); auto; discriminate.
+      pose proof (not_sle_slt dirHigh) as dirHigh'.
+      pose proof (recvmCond c_child recvm) as fromM.
+      rewrite <- fromM in dirHigh'.
+      pose proof (toParent c_child sendm dirHigh') as dM.
+      pose proof (fromChild c_child recvm dirHigh') as dM'.
+      rewrite <- dM' in dM; rewrite dM.
+      assert (le: ts <= t) by omega.
+      pose proof (sendmFrom (st c_child) sendm) as fromM'.
+      rewrite fromM' in dirHigh'.
+      assert (stCond: sle Sh (state c a ts)) by
+          (
+            destruct (state c a ts); unfold sle in *; unfold slt in *; auto;
+            discriminate).
+      assert (cond2: forall c0, parent c0 c -> sle (dir c c0 a ts) Sh) by
+          (intros c0 c0_child; unfold parent in *; destruct c; destruct c0;
+           assert (f: False) by auto; firstorder).
+      pose proof (SIHt ts le c (conj stCond cond2)) as useful.
+      destruct (data c a ts).
+      intros ti cond1.
+      assert (cond3: 0 <= ti < ts \/ ts <= ti < S t) by omega.
+      generalize noSt cond3 useful; clear; firstorder.
+      destruct useful as [cb [ib [tb [tbTs [deqTb rest]]]]].
+      exists cb; exists ib; exists tb.
+      assert (tsLeSt: ts <= S t) by omega.
+      constructor. 
+      assert (tb < S t) by omega.
+      assumption.
+      constructor. assumption.
+      intros ti cond1.
+      assert (cond3: tb < ti < ts \/ ts <= ti < S t) by omega.
+      generalize rest cond3 noSt; clear; firstorder.
+      assert (contra: forall c, parent c Parent -> ~ ~ sle (dir Parent c a t) Sh) by
+          firstorder.
+      assert (contra2: forall c, parent c Parent -> sle (dir Parent c a t) Sh) by
+          (intros c parentC;
+           specialize (contra c parentC);
+           unfold sle in *; destruct (dir Parent c a t); auto).
+      firstorder.
+
+      destruct H as [H _].
+      assert (noChildren: forall c, parent c (Child n) -> False) by
+         ( intros c c_parent; unfold parent in *; destruct c; auto ).
+      destruct (classical (sle Sh (state (Child n) a t))) as [easy|hard].
+      assert (ob: t <= t) by omega.
+      assert (contra: forall c, parent c (Child n) -> sle (dir (Child n) c a t) Sh) by
+          (generalize noChildren; clear; firstorder).
+      specialize (SIHt t ob (Child n) (conj easy contra)).
+      assert (c_child: parent (Child n) Parent) by (unfold parent; auto).
+      pose proof (conservative c_child a t) as cons.
+      pose proof (compatible a t c_child) as [_ dirLow].
+      assert (others: forall c', c' <> Child n -> leaf c' -> sle (state c' a t) Sh).
+      intros c' c'_ne leaf_c'.
+      assert (c'_child: parent c' Parent) by (unfold parent in *; unfold leaf in *; auto).
+      specialize (dirLow c' c'_ne c'_child).
+      pose proof (conservative c'_child a t) as cons2.
+      unfold sle in *; destruct (state c' a t); destruct (dir Parent c' a t);
+      destruct (state (Child n) a t); destruct (dir Parent (Child n) a t); auto.
+      assert (otherDeq: forall c', c' <> Child n -> forall li ii, ~ deqR c' li a St ii t).
+      unfold not; intros c' c'_ne li ii deqSt.
+      pose proof (deqLeaf deqSt) as c'_leaf.
+      specialize (others c' c'_ne c'_leaf).
+      pose proof (processDeq deqSt) as M; simpl in *.
+      rewrite M in others; unfold sle in others; auto.
+      destruct (classical (exists li ii, deqR (Child n) li a St ii t)) as
+          [[li [ii deqSt]]|notEx].
+      pose proof (deqImpData deqSt) as newData.
+      rewrite newData in *.
+      exists (Child n); exists ii; exists t.
+      assert (t_lt_St: t < S t) by omega.
+      constructor. assumption.
+      constructor. assumption.
+      intros ti [c1 c2].
+      assert (f: False) by omega.
+      firstorder.
+      assert (forall li ii, ~ deqR (Child n) li a St ii t) by firstorder.
+      assert (noDeq: forall c0 li ii, ~ deqR c0 li a St ii t).
+      intros c0 li ii.
+      assert ({c0 = Child n} + {c0 <> Child n}) by (decide equality; decide equality).
+      destruct H1 as [eq|neq].
+      rewrite eq in *.
+      firstorder.
+      firstorder.
+      destruct (classical (data (Child n) a (S t) = data (Child n) a t)) as [eq|neq].
+      rewrite eq.
+      destruct (data (Child n) a t).
+      intros ti cond.
+      assert (mur1: 0 <= ti < t \/ ti = t) by omega.
+      destruct mur1 as [easy2|hard].
+      apply (SIHt ti easy2).
+      rewrite hard in *; firstorder.
+      destruct SIHt as [cb [ib [tb [tbLt [deqSt rest]]]]].
+      exists cb; exists ib; exists tb.
+      constructor. assert (tb < S t) by omega. assumption.
+      constructor. assumption.
+      intros ti cond.
+      assert (mur1: tb < ti < t \/ ti = t) by omega.
+      destruct mur1 as [easy2|hard].
+      apply (rest ti easy2).
+      rewrite hard in *; firstorder.
+      pose proof (changeData neq) as [[m [fromParent|toChild]]| deqSt].
+      destruct fromParent as [p [p_parent [recvm fromM]]].
+      pose proof (recvImpMark recvm) as [ts [ts_le_t sendm]].
+      pose proof (sendmFrom (dt p_parent) sendm) as fromM'.
+      pose proof (cRecvRespPrevState p_parent recvm sendm) as same.
+      rewrite <- fromM' in same.
+      rewrite <- same in fromM.
+      rewrite fromM in easy.
+      unfold sle in easy; firstorder.
+      destruct toChild as [c' [c'_child _]].
+      unfold parent in c'_child; firstorder.
+      destruct deqSt as [l [i deqSt]].
+      pose proof (deqImpData deqSt) as newData.
+      rewrite newData.
+      assert (e1: t < S t) by omega.
+      assert (e2: forall ti, t < ti < S t -> forall ci li ii, ~ deqR ci li a St ii ti) by
+          (intros ti [cond1 cond2]; assert (f: False) by omega; firstorder).
+      generalize e1 e2 deqSt; clear; firstorder.
+      assert (inv: state (Child n) a t = In) by
+          (unfold sle in hard; destruct (state (Child n) a t); firstorder).
+      clear hard.
+      assert (upgrade: slt (state (Child n) a t) (state (Child n) a (S t))) by
+          (rewrite inv; unfold slt in *; unfold sle in *; destruct (state (Child n) a (S t));
+           auto).
+      pose proof (slt_neq' upgrade) as neq'.
+      assert (neq: state (Child n) a (S t) <> state (Child n) a t) by auto.
+      assert (c_child: parent (Child n) Parent) by (unfold parent; auto).
+      pose proof (change (st c_child) neq) as [[m markm] | [m recvm]].
+      pose proof (cSendDowngrade c_child markm) as dwn.
+      pose proof (slt_slti_false upgrade dwn) as f.
+      firstorder.
+      pose proof (recvImpMark recvm) as [ts [ts_le_t sendm]].
+
+      remember (Child n) as c.
+
+
+      assert (pHigh: forall tx, ts <= tx < S t -> ~ sle (dir Parent c a tx) In)
+        by admit.
+      assert (cLow: forall tx, ts <= tx < S t -> slt (state c a tx) Mo) by admit.
+
+
+
+
+      assert (others: forall tx, ts <= tx < S t ->
+                                 forall c', c' <> c -> parent c' Parent ->
+                                            sle (dir Parent c' a tx)
+                                                match dir Parent c a tx with
+                                                  | In => Mo
+                                                  | Sh => Sh
+                                                  | Mo => In
+                                                end) by
+          (intros tx _; apply (compatible a tx c_child)).
+      assert (c'DirLow:
+                forall tx,
+                  ts <= tx < S t -> 
+                  forall c', c' <> c -> parent c' Parent -> slt (dir Parent c' a tx) Mo).
+      intros tx cond c' c'_ne_c c'_child.
+      specialize (others tx cond c' c'_ne_c c'_child).
+      specialize (pHigh tx cond).
+      unfold slt in *; destruct (dir Parent c a tx); destruct (dir Parent c' a tx); auto.
+      assert (c'Low: forall tx, ts <= tx < S t -> forall c',
+                                                   c' <> c ->
+                                                   parent c' Parent ->
+                                                   slt (state c' a tx) Mo).
+      intros tx cond c' c'_ne_c c'_child.
+      specialize (c'DirLow tx cond c' c'_ne_c c'_child).
+      pose proof (conservative c'_child a tx) as sig.
+      unfold slt in *; destruct (dir Parent c' a tx); destruct (state c' a tx); auto.
+      assert (allLow: forall tx, ts <= tx < S t -> forall c0,
+                                           parent c0 Parent -> slt (state c0 a tx) Mo).
+      intros tx cond c0 c0_child.
+      assert (cache: {c0 = c} + {c0 <> c}) by (
+                                        decide equality;
+                                        decide equality).
+      destruct cache as [eq|notEq].
+      rewrite eq in *; apply (cLow tx cond).
+      apply (c'Low tx cond c0 notEq c0_child).
+      assert (noSt: forall ti, ts <= ti < S t ->
+                               forall ci li ii, ~ deqR ci li a St ii ti).
+      unfold not; intros ti cond ci li ii deqSt.
+      pose proof (deqLeaf deqSt) as leafCi.
+      assert(ci_child: parent ci Parent) by (unfold leaf in *; unfold parent in *; auto).
+      pose proof (processDeq deqSt) as mustMo.
+      simpl in *.
+      specialize (allLow ti cond ci ci_child).
+      unfold sle in allLow; destruct (state ci a ti); auto; discriminate.
+
+      
+      pose proof (cRecvRespPrevState c_child recvm sendm) as prevState.
+      pose proof (sendmFrom (dt c_child) sendm) as fromM.
+      rewrite <- fromM in prevState.
+      rewrite prevState in inv.
+      pose proof (fromParent c_child recvm inv) as dM.
+      pose proof (toChild c_child sendm inv) as dM'.
+      rewrite dM' in dM; rewrite dM.
+      assert (le: ts <= t) by omega.
+      assert (stCond: sle Sh (state Parent a ts)) by
+          (
+           specialize (stEq ts); rewrite stEq; unfold sle; auto).
+      pose proof (sendCCond c_child sendm) as [_ rest].
+      pose proof (recvmChange (st c_child) recvm) as newState.
+      rewrite <- newState in rest.
+      assert (cond1: forall c0, c0 <> c -> parent c0 Parent -> sle (dir Parent c0 a ts) Sh) by
+          (
+          intros c0 cond c0_child; specialize (rest c0 cond c0_child);
+          destruct (state c a (S t)); destruct (dir Parent c0 a ts);
+          unfold sle in *; unfold slt in *; auto).
+      rewrite inv in fromM.
+      assert (cond2: forall c, parent c Parent -> sle (dir Parent c a ts) Sh).
+          intros c0 c0_child; assert (H2: {c0 = c} + {c0 <> c}) by 
+                                 (decide equality; decide equality);
+          destruct H2 as [easy | hard].
+          rewrite easy in *; rewrite <- fromM; unfold sle; auto.
+          apply (cond1 c0 hard c0_child).
+      pose proof (SIHt ts le Parent (conj stCond cond2)) as useful.
+      destruct (data Parent a ts).
+      intros ti condx.
+      assert (cond3: 0 <= ti < ts \/ ts <= ti < S t) by omega.
+      generalize noSt cond3 useful; clear; firstorder.
+      destruct useful as [cb [ib [tb [tbTs [deqTb rest2]]]]].
+      exists cb; exists ib; exists tb.
+      assert (tsLeSt: ts <= S t) by omega.
+      constructor. 
+      assert (tb < S t) by omega.
+      assumption.
+      constructor. assumption.
+      intros ti condx.
+      assert (cond3: tb < ti < ts \/ ts <= ti < S t) by omega.
+      generalize rest2 cond3 noSt; clear; firstorder.
+    Qed.
+  End ForAddr.
+End LatestValueTheorems.
